Patrick Wu, Alex Zhang, Nhi Nguyen

Algo 344

HW 1

---

1. 1) 	\\[\begin{aligned}
		&f(n) = \sqrt{2^{7n}},\;g(n) = \lg{7^{2n}} \\\
		&\implies f(n) = 2^{7/2n} \\\
		&\text{L'Hopital's Rule:} \lim\_{n\to\infty}{f(n)\over g(n)} = \lim\_{n\to\infty}{f'(n)\over g'(n)} \\\
		&f'(n) = 7\*2^{{7n\over2}-1}\ln(2) \\\
		&g'(n) = {\ln(49)\over\ln(7)} \\\
		&\lim\_{n\to\infty}{f'(n)\over g'(n)}= \lim\_{n\to\infty}{7\*2^{{7n\over2}-1}\ln(2)\ln(7)\over\ln(49)} = \infty \\\
		&f(n) = \Omega(g(n)) \\\
		\end{aligned}\\]
		
	2) \\[\begin{aligned}
		&f(n) = 2^{n\ln(n)},\;g(n) = n! \\\
		&\text{Stirling's Approximation: }\ln(n!) = n\ln(n) - n + O(\ln(n)) \\\
		&\lg(n!) = {\ln(n!)\over\ln(2)} \\\
		&\lim\_{n\to\infty}{\lg f(n)\over\lg g(n)} = \lim\_{n\to\infty}{n\ln(n)\over\lg(n!)} = \lim\_{n\to\infty}{\ln(2)\;n\ln(n)\over n\ln(n) - n + O(\ln(n))} \\\
		&f'(n) = 1+\ln(n) \\\
		&g'(n) = 1+\ln(n)-1+O(1/n) = \ln(n) + O(1/n) \\\
		&\text{We can drop the O because it describes the } \\\
		&\text{upper-bound limiting behavior of its respective function} \\\
		&\lim\_{n\to\infty}{f'(n)\over g'(n)} = \lim\_{n\to\infty}{\ln(2) + \ln(2)\ln(n)\over \ln(n) + 1/n} = \ln(2) \\\
		&f(n) = \Theta(g(n))
		\end{aligned}\\]
		
	3)	\\[\begin{aligned}
		&f(n) = \lg(\lg^*n),\;g(n) = \lg^\*\lg(n) \\\
		&\lg^\*n = 1+\lg^\*\lg(n) \\\
		&\lg^\*\lg(n) = \lg^\*n - 1 \\\
		&\text{for } x = lg^\*n \\\
		&\lim_{n\to\infty}{\lg(x)\over x-1} = 0 \\\
		&f(n) = O(g(n)) \\\
		\end{aligned}\\]
	
	4) \\[\begin{aligned}
		&f(n)={\lg(n^2)\over n},\;g(n) = \lg^\*n \\\
		&\lim\_{n\to\infty}{\lg(n^2)\over n\lg^\*n} = \lim\_{n\to\infty}{\lg(n^2)\over n + n\lg^\*\lg(n)} \\\
		&\implies \lim\_{n\to\infty}{\lg(n^2)\over n} \\\
		&f'(n) = {2n\over n^2\ln(2)} \\\
		&\lim\_{n\to\infty}{2n\over n^2\ln(2)} = 0 \\\
		&f(n) = O(g(n)) \\\
		\end{aligned}\\]
	
	5) \\[\begin{aligned}
		&f(n)=2^n,\;g(n)=n^{\lg(n)} \\\
		&\lg(2^n) = n,\;\lg(n^{\lg(n)}) = (\lg n)^2 \\\
		&f'(n) = 1,\;g'(n) = {2(\lg n)\over n\ln 2} \\\
		&\lim\_{n\to\infty}{\ln 2(n)\over 2(\lg n)} = \infty \\\
		&f(n) = \Omega(g(n))
		\end{aligned}\\]
		
	6) \\[\begin{aligned}
		&f(n) = 2^{\sqrt{\lg n}},\;g(n) = n(\lg n)^3 \\\
		&\lg f(n) = (\lg n)^Â½,\;\lg g(n) = \lg n + 3\lg\lg n \\\
		&f'(n) = {\lg n\over n\ln 2} \\\
		&g'(n) = {1\over n\ln 2} + {3\over n \ln 2\ln n} = {3\ln n\over n\ln 2\ln n} \\\
		&\lim\_{n\to\infty}{f'(n)\over g'(n)} = {\lg n(n\ln 2)(\ln n)\over 3\ln n(n\ln 2)} \\\
		&\implies\lim\_{n\to\infty}{\lg n\over 3} = \infty \\\
		&f(n) = \Omega(g(n)) \\\
		\end{aligned}\\]
		
	7) \\[\begin{aligned}
		&f(n)=e^{\cos(n)},\;g(n)=\lg n \\\
		&f(n)\text{ is harmonic and } \\\
		&g(n)\text{ is monotonically increasing.} \\\
		&f(n) = O(g(n)) \\\
		\end{aligned}\\]
		
	8) \\[\begin{aligned}
		&f(n) = \lg n^2 = 2\lg n \\\
		&g(n) = (\lg n)^2 \\\
		&\lim\_{n\to\infty}{2\lg n\over\lg n^2} = \lim\_{n\to\infty}{2\over\lg n} = 0\\\
		&f(n) = O(g(n)) \\\
		\end{aligned}\\]
		
	9) \\[\begin{aligned}
		&f(n) = \sqrt{4n^2-12n+9},\;g(n)=n^{3/2} \\\
		&f(n)^2 = 4n^2-12n+9,\;g(n)^2=n^3 \\\
		&\lim\_{n\to\infty}{4n^2-12n+9\over n^3} = 0 \\\
		&f(n) = O(g(n)) \\\
		\end{aligned}\\]
		
	10) \\[\begin{aligned}
		f(n)=\sum_{k=1}^nk,\;g(n)=(n+2)^2 \\\
		\lim\_{n\to\infty}\sum\_{k=1}^nk = \infty \\\
		\end{aligned}\\]
2.  1. $$$O(n)$$$ 
	2. $$$O(n^2)$$$
	3. $$$O(n)$$$
	4. $$$O(n^2)$$$
	5. $$$m$$$ times
	6. $$$O(n^3)$$$
	7. $$$O(1)$$$
	8. $$$O(n^2)$$$
	9. $$$O(n^2)$$$
	10. $$$m$$$ times
	11. $$$O(n^2)$$$
	12. $$$O(n^2)$$$
	13. $$$O(n^2)$$$
	14. $$$O(n^2)$$$
	15. $$$O(n^2)$$$
	
3.  a.) tree datastructure m = children every node can have (at most) N = # nodes tree can have
	Lower bound for height of tree? (tree must be at least __ tall)
	if $$$m=1, N=3$$$, then $$$h=2$$$
	$$$m=2, N=3,$$$ then $$$h=1$$$
	$$$m=3, N=4$$$, then $$$h=4$$$ 
	$$$m=x,\; N=x+1$$$, then $$$h=1$$$	How did we get height? $$$m=x$$$	$$$N = x-1$$$	$$$\to h = 1$$$	1 of N will be the root of the tree	How to have the smallest height? Every level is filled to capacity or not 	filled    
    $$$h = \log(m, N)$$$b.)\\[\begin{aligned}     h(m) = \log(m, N) \\\
	h(m') = \log(m', N) \\\	= \log(m, N) / \log(m', N) \\\	\log(m,N) / (\log(m,N) / \log(m, m')) \\\	\to \log(m, m')
	\end{aligned}\\]	$$$\text{constant as long as }m=m'$$$
		
4.  a) \\[\begin{aligned}
		a^{b-1}\bmod b &= 1 \\\
		2^{902} &= 2^{900}*2^2 \\\
		&= (2^6)^150 * 2^2 \\\
		&= (2^6\bmod 7)^150 * 2^2\bmod 7 \\\
		&= 1\*4 = 4 \\\
		\end{aligned}\\]
	b)	1)	\\[\begin{aligned}
			11^{-1}\bmod 120 = x \\\
			\implies 11x = 1\bmod 120 \\\
			\implies \gcd(120, 11) = 120\bmod 11 = 10 \\\
			\gcd(11, 10) = 1 \\\
			10 + 1 = 11 \\\
			\end{aligned}\\]
		2) \\[\begin{aligned}
			13^{-1}\bmod45 = x \\\
			13x = 1\bmod45 \\\
			\gcd(45,13)\implies 45\bmod13=6 \\\
			\gcd(13,6)\implies 13\bmod6=1 \\\
			6+1=7 \\\
			\end{aligned}\\]
		3) \\[\begin{aligned}
			35^{-1}\bmod77=x \\\
			35x=1\bmod77 \\\
			\gcd(77,35)\implies 77\bmod35 = 7 \\\
			\gcd(35,7)\implies 35\bmod7 = 0 \\\
			7+0=7 \\\
			\end{aligned}\\]
		4) \\[\begin{align}
			9^{-1}\bmod11=x \\\
			9x = 1\bmod11 \\\
			\gcd(11,9)\implies 11\bmod 9 = 2 \\\
			\gcd(9,2)\implies 9\bmod2 = 1 \\\
			2+1=3 \\\
			\end{align}\\]
		5) \\[\begin{aligned}
			11^{-1}\bmod1111 \\\
			11x=1\bmod1111 \\\
			\gcd(1111,11)\implies 1111\bmod11 = 0 \\\
			\text{Not invertible. } \\\
			x\text{ is inverse modulo }n \iff x \text{ is coprime to n.} \\\
			\end{aligned}\\]
			
5.  a) \\[\begin{aligned}
		\gcd(5x+3y, 3x+2y)\\\
		&= 5x+3y\bmod 3x+2y \\\
		&= 2x+y \\\
		\gcd(3x+2y, 2x+y)\\\
		&= x+y \\\
		\gcd(2x+y, x+y)\\\
		&= x \\\
		\gcd(x+y, x)\\\
		&= y \\\
		\gcd(x, y)\\\
		&= x-y \\\
		\text{True.} \\\
		\end{aligned}\\]
	b) \\[\begin{aligned}
		S_i=1+\prod_{i=0}^{n-1}S_i, S_0 = 2 \\\
		S_1 = 1+2 = 3 \\\
		S_2 = 1 + 2\*3 = 7 \\\
		S_3 = 1 + 2\*3\*7 = 43 \\\
		S_4 = 1 + 2\*3\*7\*43 = 1807 \\\
		\vdots\quad\text{and so on}
		\end{aligned}\\]
This series of numbers is actually known as Sylvester's Sequence, which is a sequence where each term is the product of a preceding term PLUS one. This sequence comes from Euclid's proof that there is an infinite number of primes and no two terms share a prime factor. Since no two terms share a prime factor and this sequence consists of ONLY prime numbers, we can safely say that each term is only divisible by itself and 1. We can then say that if we have terms x and y from this sequence, then gcd(x,y)=1, or the only number that evenly divides x and y is 1. Thus, if we picked any two terms from this sequence, we can safely say that these terms are relatively prime to each other.		